veric/SeparationLogic.v
@@ -1175,9 +1175,15 @@ forall Espec ts x,
       (frame_ret_assert (function_body_ret_assert (fn_return f) (Q ts x)) (stackframe_of f))
 end.
 
+Definition Pre_is_Lvar_Closed (spec:funspec) :=
+  match spec with mk_funspec _ _ _ P _ _ _ => 
+    forall ts x, closed_wrt_lvars (fun i => True) (P ts x)
+end.
+              
 Definition semax_body
    (V: varspecs) (G: funspecs) {C: compspecs} (f: function) (spec: ident * funspec): Prop :=
-exists spec', funspec_sub spec' (snd spec) /\ 
+Pre_is_Lvar_Closed (snd spec) /\
+exists spec', funspec_sub spec' (snd spec) /\
               @semax_body_orig V G C f (fst spec, spec') .
 
 Definition semax_prog
@@ -1229,7 +1235,7 @@ Axiom semax_func_nil:   forall {Espec: OracleKind},
         forall V G C ge, @semax_func Espec V G C ge nil nil.
 
 Axiom semax_func_cons:
-  forall {Espec: OracleKind},
+  forall {Espec: OracleKind}, (*
      forall fs id f fsig cc A P Q NEP NEQ (V: varspecs) (G G': funspecs) {C: compspecs} ge b,
       andb (id_in_list id (map (@fst _ _) G))
       (andb (negb (id_in_list id (map (@fst ident fundef) fs)))
@@ -1244,7 +1250,24 @@ Axiom semax_func_cons:
       semax_body V G f (id, mk_funspec fsig cc A P Q NEP NEQ)->
       semax_func V G ge fs G' ->
       semax_func V G ge ((id, Internal f)::fs)
-           ((id, mk_funspec fsig cc A P Q NEP NEQ)  :: G').
+           ((id, mk_funspec fsig cc A P Q NEP NEQ)  :: G').*)
+   forall  fs id f fsig cc A P Q NEP NEQ (V: varspecs) (G G': funspecs) {C: compspecs} ge b,
+  andb (id_in_list id (map (@fst _ _) G))
+  (andb (negb (id_in_list id (map (@fst ident fundef) fs)))
+    (semax_body_params_ok f)) = true ->
+  Forall
+     (fun it : ident * type =>
+      complete_type cenv_cs (snd it) =
+      true) (fn_vars f) ->
+   var_sizes_ok (f.(fn_vars)) ->
+   f.(fn_callconv) = cc ->
+   Genv.find_symbol ge id = Some b -> 
+   Genv.find_funct_ptr ge b = Some (Internal f) -> 
+  semax_body V G f (id, mk_funspec fsig cc A P Q NEP NEQ) ->
+  semax_func V G ge fs G' ->
+  (*Now part of semax_body: (forall ts x, closed_wrt_lvars (fun i => True) (P ts x)) ->*)
+  semax_func V G ge ((id, Internal f)::fs)
+       ((id, mk_funspec fsig cc A P Q NEP NEQ)  :: G').
 
 Axiom semax_func_cons_ext:
   forall {Espec: OracleKind},
